---
title: "Homework 7"
author: "Raul Torres Aragon"
date: "11/3/2023"
output: pdf_document
---

```{r setup, include=FALSE}
knitr::opts_chunk$set(echo = TRUE)
df <- faithful
colors <- c("#1B9E77","#D95F02","#7570B3","#E7298A")
#load("hw7_en.Rdata")
```

```{r, fig.align='center', out.width="64%", echo=FALSE}
#knitr::include_graphics("hw5_table1.png")
```  

# Q1  

Load the dataset *faithful* on R. Then:  

## (a)  
Estimate and plot the density of `faithful$eruptions`  
```{r q1a, fig.align='center', out.width="64%", echo=TRUE}
plot(density(df$eruptions), lwd = 2,
     main="Desnsity estimation of Faithful eruptions")
```  

### (b)  
Create a new plot and superimpose different density estimations with bandwidths equal to 0.1, 0.5, 1.0.  
```{r q1b, fig.align='center', out.width="64%", echo=TRUE}
plot(density(df$eruptions), lwd = 2,
     main="Desnsity estimation of Faithful eruptions")
density(df$eruptions, bw = 0.1) |> lines(col = colors[1])
density(df$eruptions, bw = 0.5) |> lines(col = colors[2])
density(df$eruptions, bw = 1.0) |> lines(col = colors[3])
legend("topright", 
       title="Bandwidth",
       legend=c("0.34", "0.1", "0.5", "1.0"),  
       fill = c("black",colors[1:3]),
       cex = 0.6)
```  


### (c)  
Get the density estimate at exactly point $x = 3.1$ using $h=0.15$ and the Epanechnikov.  

```{r q1c, fig.align='center', out.width="64%", echo=FALSE}
dens_est <- density(df$eruptions, kernel = "epanechnikov", bw = 0.15)
dens_est_x <- mean(dens_est$y[dens_est$x>3.091 & dens_est$x<=3.109])
plot(density(df$eruptions, kernel = "epanechnikov", bw = 0.15), 
     lwd = 2,
     main="Desnsity estimation ((Epanechnikov kernel) of Faithful eruptions",
     xlab="eruptions")
abline(v = 3.1, col="red")
abline(h = mean(dens_est$y[dens_est$x>3.09 & dens_est$x<=3.11]), col="red")
```  

The density estimate at $x=3.1$ is `r round(dens_est_x, 3)`.  


# Q2  
Show that if $f(x)$ is normal $N(\mu, \sigma^2)$, then  
$$
\beta(f) = \int f''(x)^2dx = \frac{3\sigma^{-5}}{8\sqrt{\pi}}
$$    

First, note that for $x\sim N(\mu, \sigma^2)$, we can get its pdf, as well as its pdf's first and second derivative w.r.t. x:  

$$
\begin{aligned} 
f(x) &= \frac{1}{\sqrt{2\pi \sigma^2}}e^{\{\frac{1}{2\sigma^2} (x-\mu)^2\}}  \\
f'(x) &= \frac{1}{\sqrt{2\pi \sigma^2}} e^{\{\frac{1}{2\sigma^2} (x-\mu)^2\}} \frac{d}{dx}\bigg[ -\frac{1}{2}\frac{(x-\mu)^2}{2\sigma^2}\bigg] \\
&= -\frac{(x-\mu)}{\sigma^2} f(x) \\
f''(x) &= \bigg[-\frac{(x-\mu)}{\sigma^2}\bigg] f'(x) + f(x)-\frac{1}{\sigma^2} \\
&= f(x) \bigg[-\frac{(x-\mu)^2}{\sigma^4} - \frac{1}{\sigma^2}\bigg]
\end{aligned}
$$  
Squaring $f''(x)$ yields:  

$$
\frac{1}{2\pi\sigma^2} e^{-\frac{(x-\mu)^2}{\sigma^2}}\bigg[\frac{(x-\mu)^4}{\sigma^4}-\frac{(x-\mu)^2}{\sigma^4} + \frac{1}{\sigma^4}\bigg]
$$  

Recall that the $n$ central moment of the normal distribution is:  
$$
\sigma^n\int_{-\infty}^{\infty} \frac{1}{\sqrt{2\pi}}u^ne^{-\frac{u^2}{2}}du
$$  
where $u = (x-\mu)/\sigma$.  

Thus, integrating $f''(x)^2$, we obtain the following expression:  

$$
\int_{-\infty}^{\infty}\frac{1}{2\pi\sigma^2}e^{u^2}u^2du - \frac{1}{\pi \sigma^2} 
\int_{-\infty}^{\infty}e^uu^2/\sigma^2 du + \frac{1}{2\pi\sigma^6}
\int_{-\infty}^{\infty} e^u du
$$  
After manipulating constants to express the above in terms of $f(x)$s, we can see that the first and third term are the variance and kurtosis of the normal distribution.  

Thus,

$$
f''(x)^2 = \frac{3}{8}\frac{1}{\sigma^5\sqrt{\pi}} 
$$  
as desired. 

Show explicitly that using a Gaussian kernel leads to the "normal reference rule-of-thumb" optimal bandwidth  
$$
h_{opt} = \bigg( \frac{4}{3n} \bigg)^{1/5} \sigma \approx 1.06\sigma n^{-1/5}
$$  

The asymptotic optimal bandwidth is obtained by:  

$$
\begin{aligned}
\frac{d}{dh} AMISE(\hat{f}(x)) = h^3\kappa_2^2\beta(f)-\frac{R(K)}{nh^2}
\end{aligned}
$$  
where $R(K) = \int K(z)^2dz$ and $\kappa_2$ is the variance of the kernel.  

Solving for $h$ we get,

$$
h_{opt}^5 = \frac{R(K)\kappa^{-2}_2}{\beta(f)n}
$$  

and substituting $\kappa_2 = \sigma$ (because we're using the Gaussian kernel) and $\beta(f) = \frac{3}{8\sqrt{\pi}\sigma^5}$ per above yields:  

$$
\begin{aligned}
h_{opt} &= \bigg[ \frac{R(K)\kappa_2^{-2}}{\beta(f)n} \bigg]^{1/5} \\
&= \bigg[\frac{\int k(z^2)dz / \sigma}{3n/8\sigma^5\sqrt{\pi}} \bigg]^{1/5} \\
&= \bigg[\frac{8\sigma^5\sqrt{\pi} \int k(z^2)dz}{3n\sigma} \bigg]^{1/5} \\
&= \bigg[ \frac{8 \sigma^5 \sqrt{\pi}(2\sqrt{\pi\sigma^2})^{-1}\int e^{z^2/2}dz}{3n\sigma} \bigg]^{1/5} \\
&= \bigg[ \frac{4\sigma^5}{3n} \bigg]^{1/5} \\
&= \bigg[ \frac{4}{3n}\bigg]^{1/5}\sigma \\
&\approx 1.06 \sigma n^{-1/5}
\end{aligned} 
$$  
where $z = (x-\mu)/\sigma$.  


# Q3  

Find the quadratic spline interpolant for the data below:  
```{r, fig.align='center', out.width="37%", echo=FALSE}
knitr::include_graphics("hw7_table1.png")
```  

by assuming $z_0=0$  

We want a quadratic polynomials $Q_i(x)$ passing through the above points. 
Thus, we want:  
$$
Q_i(x) = a_ix^2 + b_ix + c_i = y_i
$$  
this yields six equations. $Q_0(x)=y_0, Q_1(x)=y_1, \dots Q_5(x)=y_5$.  

We also want continuity in $Q_i'(x)$ which means:  
$$
Q_i'(x) = 2a_ix+b_i := 2a_{i+1}x+b_{i+1} = Q_{i+1}'(x)
$$  
This yields 5 equations: $Q_0'(x_{i+1}) = Q_1'(x_i)$, $Q_1'(x_{i+1}) = Q_2'(x_i)$, ... $Q_4'(x_{i+1}) = Q_5'(x_i)$.  

The last condition is $Q_0''(x_0)=z_0$.  
Together, this system of equations, allows us to obtain coefficients $a_i$, $b_i$, and $c_i$ of each $Q_i(x)$.  

The following R code implements recursive expression for finding $Q_i'(x_i)=z_i$ starting from $z_0=0$.  

$$
z_{i+1} = -z_i + 2 \bigg( \frac{y_{i+1}-y_i}{x_{i+1}-x_i} \bigg)
$$

```{r}
X = c(-1, 0, 0.5, 1, 2, 5/2)
Y = c( 2, 1, 0.0, 1, 2, 3.0)

getZ <- function(X,Y, z0 = 0) {
  Z <- vector(mode = "numeric", length = length(Y))
  Z[1] <- z0
  for(i in 1:(length(Y)-1)){
    Z[i+1] = -Z[i] + 2 * (Y[i+1] - Y[i])/(X[i+1] - X[i])
  }
  Z
}
Z <- getZ(X, Y, z0=0)
```  

Hence, $\boldsymbol{Z}$ = `r Z`, which then allows us to obtain $Q_i(x)$ as follows:  
$$
Q_i(x) = \frac{z_{i+1}-z_i}{2(x_{i+1}-x_i)}(x-x_i)^2+z_i(x-x_i)+y_i
$$  
So,
$$
\begin{aligned}
Q_0(x) &= (x+1)^2+y_0 \\
Q_1(x) &= -2x+y_1\\
Q_2(x) &=  8(x-1/2)^2 -2(x-1/2)+ y_2\\
Q_3(x) &= -5(x-1)^2 + 6(x-1) + y_3 \\
Q_4(x) &= 12(x-2)^2 -4(x-2) +y_4
\end{aligned}
$$

# Q4  

Determine if the function below is a quadratic spline. Explain why or why not.  

```{r fig.align='center', out.width="36%", echo=FALSE}
knitr::include_graphics("hw7_functionQ.png")
```

For $Q(x)$ to be a quadratic spline, these conditions must hold:  

- $Q$ is a polynomial of at most 2nd degree on each subinterval. This holds.  
- $Q$ and $Q'$ are continuous on $(-\infty, \infty)$. Note:  
$$
\begin{aligned}
Q_0(1) = Q_1'(1) = 1 \\
Q_1(2) = Q_2(2) = 4 \\
Q_0'(1) = 1, \text{ but } Q_1'(1) = 2 \\
Q_1'(2) = Q_2'(2) = 4
\end{aligned}
$$  

So, because $Q_0'(1) \neq Q_1'(1)$ (not continuous at interior point $x=1$), $Q(x)$ is not a quadratic spline.  


# Q5  

Determine the parameters $a, b, c, d$ and $e$ so that $S$ is a natural cubic spline.  
```{r fig.align='center', out.width="49%", echo=FALSE}
knitr::include_graphics("hw7_functionSx5.png")
```

For $S$ to be a cubic spline, we must have continuity at inner points for $S, S', S''$. Hence,

$$
\begin{aligned}
S_0(1) = S_1(1) &\implies a = e -1 \\
S_0'(1)= S_1'(1) &\implies b = 2e \\
S_0''(1) = S_1''(1) &\implies c = e \\
\end{aligned}
$$  
We also have, for natural cubic splines  
$$
\begin{aligned}
0=S_0''(0) &\implies d = c/3 \\
0=S_1''(2) &\implies e = -3
\end{aligned}
$$  
Combining the expression from the cubic spline conditions yields:  
$$
\begin{aligned}
a &= -4 \\
b &= -6 \\
c &= -3 \\
d &= -1 \\
e &= -3
\end{aligned}
$$  

# Q6  
Determine the coefficients so that the function  
```{r fig.align='center', out.width="49%", echo=FALSE}
knitr::include_graphics("hw7_functionSx6.png")
```
is a cubic spline and has property $S_1'''(x)=12$.  

From the continuity conditions, as above, we have:  
$$
\begin{aligned}
S_0(1) = S_1(1) &\implies a + b + c + d = 2 \\
S_0'(1) = S_1'(1) &\implies b + 2c + 3d = 5 \\
S_0''(1) = S_1''(1) &\implies 2c + 6d = 8 \\ 
\end{aligned} 
$$  
And from property $S'''_1(x)=12$, we get $d=2$.  
Thus,  
$$
\begin{aligned}
a &= -1 \\
b &= 3 \\
c &= -2 \\
d &= 2
\end{aligned}
$$